ts: WIP finsets...?

CTL/Satisfaction.lean
@@ -1,23 +1,30 @@
+import Mathlib.Tactic.DeriveFintype
+
 import TS.Basic
 
 namespace CTL
 class StateSatisfiable (α : (p : Type) → Type) where
-  StateSat : [Fintype s] → [Model p s μ] → (m : μ p s)
+  StateSat : [Fintype s] → [DecidableEq s] → [Model p s μ] → (m : μ p s)
            → (Φ : α p)
            → (st : s)
            → Prop
 
-variable [Fintype s] [Model p s μ] (m : μ p s)
-         [StateSatisfiable α] [StateSatisfiable β]
-         (Φ : α p) (Ψ : β p)
+variable [Fintype s] [DecidableEq s] [Model p s μ] (m : μ p s)
+         [StateSatisfiable α] (Φ : α p)
 
 -- Sat(Φ) : Type
 @[simp]
 def SatState :=
   { st : s // StateSatisfiable.StateSat m Φ st }
--- Sat(Φ) : Set s
+
+variable [DecidablePred (StateSatisfiable.StateSat m Φ)]
+instance : Fintype (SatState m Φ) where
+  elems    := Finset.subtype _ (Fintype.elems)
+  complete := fun ⟨st, _⟩ => by simp; apply Fintype.complete
+
+-- Sat(Φ) : Finset s
 def setOfSatStates :=
-  @Set.range s (SatState m Φ) Subtype.val
+  @Finset.image (SatState m Φ) s _ Subtype.val Finset.univ
 
 -- TS ⊨ Φ
 @[simp]
@@ -30,12 +37,13 @@ theorem Sat_iff_initial_subset
   by
     apply Iff.intro
     . intro sat st mem
-      exact Set.mem_range_self (⟨st, sat st mem⟩ : SatState m Φ)
+      simp only [setOfSatStates]
+      -- exact Set.mem_range_self (⟨st, sat st mem⟩ : SatState m Φ)
     . intro sub st mem
       specialize sub mem
       unfold setOfSatStates at sub
-      rw [Set.mem_range] at sub
-      obtain ⟨stSat, refl⟩ := sub
-      rw [← refl]
-      exact Subtype.property stSat
+      -- rw [Set.mem_range] at sub
+      -- obtain ⟨stSat, refl⟩ := sub
+      -- rw [← refl]
+      -- exact Subtype.property stSat
 end CTL
