CTL/Basic.lean
@@ -54,7 +54,7 @@ namespace Syntax
 end Syntax
 
 section Satisfaction
-variable [Fintype s] [Model p s μ] (m : μ p s)
+variable [Fintype s] [DecidableEq s] [Model p s μ] (m : μ p s)
 
 mutual
   -- s ⊨ Φ
@@ -93,7 +93,7 @@ section Equiv
 theorem conj_congr (h₁ : Equiv Φ₁ Φ₁') (h₂ : Equiv Φ₂ Φ₂') : Equiv (Φ₁ ⬝∧ Φ₂) (Φ₁' ⬝∧ Φ₂') := by
   simp only [Equiv, setOfSatStates, SatState, StateSatisfiable.StateSat, StateSat,
              Set.ext_iff, Subtype.range_coe_subtype, Set.mem_setOf_eq] at *
-  intros _ _ _ _ _ _
+  intros _ _ _ _ _ _ _
   constructor
   . rintro ⟨sat₁, sat₂⟩; constructor; exact (h₁ _).1 sat₁; exact (h₂ _).1 sat₂
   . rintro ⟨sat₁, sat₂⟩; constructor; exact (h₁ _).2 sat₁; exact (h₂ _).2 sat₂
@@ -102,7 +102,7 @@ theorem conj_congr (h₁ : Equiv Φ₁ Φ₁') (h₂ : Equiv Φ₂ Φ₂') : Equ
 theorem neg_congr (h : Equiv Φ Φ') : Equiv (⬝¬Φ) (⬝¬Φ') := by
   simp only [Equiv, setOfSatStates, SatState, StateSatisfiable.StateSat, StateSat,
              Set.ext_iff, Subtype.range_coe_subtype, Set.mem_setOf_eq] at *
-  intros _ _ _ _ _ _
+  intros _ _ _ _ _ _ _
   constructor
   . rintro negSat sat; exact negSat ((h _).2 sat)
   . rintro negSat sat; exact negSat ((h _).1 sat)
@@ -111,7 +111,7 @@ theorem neg_congr (h : Equiv Φ Φ') : Equiv (⬝¬Φ) (⬝¬Φ') := by
 theorem exist_next_congr (h : Equiv Φ Φ') : Equiv (⬝∃⬝◯Φ) (⬝∃⬝◯Φ') := by
   simp only [Equiv, setOfSatStates, SatState, StateSatisfiable.StateSat, StateSat, PathSat,
              Set.ext_iff, Subtype.range_coe_subtype, Set.mem_setOf_eq] at *
-  intros _ _ _ _ _ _
+  intros _ _ _ _ _ _ _
   constructor
   . rintro ⟨π, sat⟩; exact ⟨π, (h _).1 sat⟩
   . rintro ⟨π, sat⟩; exact ⟨π, (h _).2 sat⟩
@@ -121,7 +121,7 @@ set_option maxHeartbeats 1000000 in
 theorem exist_untl_congr (h₁ : Equiv Φ Φ') (h₂ : Equiv Ψ Ψ') : Equiv (⬝∃(Φ ⬝U Ψ)) (⬝∃(Φ' ⬝U Ψ')) := by
   simp only [Equiv, setOfSatStates, SatState, StateSatisfiable.StateSat, StateSat, PathSat,
              Set.ext_iff, Subtype.range_coe_subtype, Set.mem_setOf_eq] at *
-  intros _ _ _ _ _ _
+  intros _ _ _ _ _ _ _
   constructor
   . rintro ⟨π, j, satJ, satK⟩; exact ⟨π, j, (h₂ _).1 satJ, fun k => (h₁ _).1 (satK k)⟩
   . rintro ⟨π, j, satJ, satK⟩; exact ⟨π, j, (h₂ _).2 satJ, fun k => (h₁ _).2 (satK k)⟩
@@ -130,7 +130,7 @@ theorem exist_untl_congr (h₁ : Equiv Φ Φ') (h₂ : Equiv Ψ Ψ') : Equiv (�
 theorem all_next_congr (h : Equiv Φ Φ') : Equiv (⬝∀⬝◯Φ) (⬝∀⬝◯Φ') := by
   simp only [Equiv, setOfSatStates, SatState, StateSatisfiable.StateSat, StateSat, PathSat,
              Set.ext_iff, Subtype.range_coe_subtype, Set.mem_setOf_eq] at *
-  intros _ _ _ _ _ _
+  intros _ _ _ _ _ _ _
   constructor
   . rintro sat π; rw [←h]; exact sat π
   . rintro sat π; rw [h] ; exact sat π
@@ -140,7 +140,7 @@ theorem all_next_congr (h : Equiv Φ Φ') : Equiv (⬝∀⬝◯Φ) (⬝∀⬝◯
 theorem all_untl_congr (h₁ : Equiv Φ Φ') (h₂ : Equiv Ψ Ψ') : Equiv (⬝∀(Φ ⬝U Ψ)) (⬝∀(Φ' ⬝U Ψ')) := by
   simp only [Equiv, setOfSatStates, SatState, StateSatisfiable.StateSat, StateSat, PathSat,
              Set.ext_iff, Subtype.range_coe_subtype, Set.mem_setOf_eq] at *
-  intros _ _ _ _ _ _
+  intros _ _ _ _ _ _ _
   constructor
   . rintro sat π; obtain ⟨j, ⟨satJ, satK⟩⟩ := sat π; exact ⟨j, ⟨(h₂ _).1 satJ, fun k => (h₁ _).1 (satK k)⟩⟩
   . rintro sat π; obtain ⟨j, ⟨satJ, satK⟩⟩ := sat π; exact ⟨j, ⟨(h₂ _).2 satJ, fun k => (h₁ _).2 (satK k)⟩⟩
