TS/Finset.lean
@@ -1,0 +1,11 @@
+import Mathlib.Data.Finset.Basic
+
+open Std.ExtendedBinder Finset
+
+syntax "[" extBinder " | " term "]" : term
+
+open Lean Elab Term in
+elab_rules : term
+  | `([ $x:ident | $p ])      => do elabTerm (← `(filter (fun $x:ident ↦ $p) univ)) none
+  | `([ $x:ident : $t | $p ]) => do elabTerm (← `(filter (fun $x:ident :$t ↦ $p) univ)) none
+  | `([ $x:ident ∈ $s | $p ]) => do elabTerm (← `(filter (fun $x:ident ↦ $p) $s)) none
